theories/properties.v
@@ -1015,571 +1015,70 @@ Ltac extract_listn :=
   | H: _ :: _ = _ ++ _ |- _ => symmetry in H
          end.
 
-Lemma value_subtyping_eq: forall t,
-    t <t: t.
-Proof.
-  move => t.
-  unfold value_subtyping => /=.
-  rewrite eq_refl.
-  by lias.
-Qed.
-
-Lemma value_subtyping_trans: forall t1 t2 t3,
-    t1 <t: t2 ->
-    t2 <t: t3 ->
-    t1 <t: t3.
-Proof.
-  unfold value_subtyping.
-  move => t1 t2 t3 Hs1 Hs2; remove_bools_options; subst; rewrite eq_refl; by lias.
-Qed.
-
-Lemma values_subtyping_eq: forall ts,
-    ts <ts: ts.
-Proof.
-  induction ts => //=.
-  by rewrite value_subtyping_eq.
-Qed.
-
-Lemma values_subtyping_size: forall ts1 ts2,
-    ts1 <ts: ts2 ->
-    size ts1 = size ts2.
-Proof.
-  move => ts1 ts2 Hsub.
-  by apply all2_size in Hsub.
-Qed.
-
-Lemma values_subtyping_trans: forall ts1 ts2 ts3,
-    ts1 <ts: ts2 ->
-    ts2 <ts: ts3 ->
-    ts1 <ts: ts3.
-Proof.
-  induction ts1 as [ | x ts1]; destruct ts2 as [ | y ts2] => //; destruct ts3 as [ | z ts3] => //=; move => Hs1 Hs2; remove_bools_options.
-  by erewrite value_subtyping_trans; eauto.
-Qed.
-
-Lemma values_subtyping_cat_trans: forall ts1 ts2 ts3 ts4,
-    ts1 <ts: ts2 ->
-    (ts2 ++ ts3) <ts: ts4 ->
-    (ts1 ++ ts3) <ts: ts4.                        
-Proof.
-  induction ts1 as [ | x ts1]; destruct ts2 as [ | y ts2]; destruct ts4 as [ | z ts4] => //=.
-  move => Hsub1 Hsub2; remove_bools_options.
-  by erewrite value_subtyping_trans; eauto.
-Qed.
-
-Lemma values_subtyping_cat: forall tx1 tx2 ty1 ty2,
-  size tx1 = size ty1 ->  
-  (tx1 ++ tx2) <ts: (ty1 ++ ty2) = (tx1 <ts: ty1) && (tx2 <ts: ty2).
-Proof.
-  move => tx1 tx2 ty1 ty2 Hsize.
-  unfold values_subtyping.
-  by rewrite all2_cat => //.
-Qed.
-
-Lemma values_subtyping_split1: forall ts ts1 ts2,
-    ts <ts: (ts1 ++ ts2) ->
-    ((take (size ts1) ts) <ts: ts1) && ((drop (size ts1) ts) <ts: ts2).
-Proof.
-  move => ts ts1 ts2; unfold values_subtyping.
-  by apply all2_split1.
-Qed.
-
-Lemma values_subtyping_split2: forall ts ts1 ts2,
-    (ts1 ++ ts2) <ts: ts ->
-    (ts1 <ts: (take (size ts1) ts)) && (ts2 <ts: (drop (size ts1) ts)).
-Proof.
-  move => ts ts1 ts2; unfold values_subtyping.
-  by apply all2_split2.
-Qed.
-
-Lemma values_subtyping_split: forall ts1 ts2 n,
-    n <= size ts1 ->
-    (ts1 <ts: ts2) ->
-    ((take n ts1) <ts: (take n ts2)) /\
-    ((drop n ts1) <ts: (drop n ts2)).
-Proof.
-  move => ts1 ts2 n Hbound Hsub.
-  rewrite - (cat_take_drop n ts1) in Hsub.
-  apply values_subtyping_split2 in Hsub; remove_bools_options.
-  rewrite size_takel in H => //.
-  by rewrite size_takel in H0.
-Qed.
-  
-Lemma func_subtyping_eq: forall tf,
-    tf <tf: tf.
-Proof.
-  move => [ts1 ts2].
-  unfold func_subtyping.
-  repeat split => //; by apply values_subtyping_eq.
-Qed.
-
-Lemma func_subtyping_trans: forall tf1 tf2 tf3,
-    tf1 <tf: tf2 ->
-    tf2 <tf: tf3 ->
-    tf1 <tf: tf3.
-Proof.
-  move => [tx1 ty1] [tx2 ty2] [tx3 ty3].
-  unfold func_subtyping.
-  move => [??] [??].
-  split; by eapply values_subtyping_trans; eauto.
-Qed.
-
-Lemma instr_subtyping_eq: forall tf,
-    tf <ti: tf.
-Proof.
-  move => [ts1 ts2].
-  unfold instr_subtyping.
-  exists nil, nil, ts1, ts2; repeat split => //; by apply values_subtyping_eq.
-Qed.
-
-Lemma instr_subtyping_trans: forall tf1 tf2 tf3,
-    tf1 <ti: tf2 ->
-    tf2 <ti: tf3 ->
-    tf1 <ti: tf3.
-Proof.
-  move => [tx1 ty1] [tx2 ty2] [tx3 ty3].
-  unfold instr_subtyping.
-  move => [ts1 [ts1' [tsubx12 [tsuby12 [-> [-> [Hsub1 [Hsubx1 Hsuby1]]]]]]]].
-  move => [ts2 [ts2' [tsubx23 [tsuby23 [-> [-> [Hsub2 [Hsubx2 Hsuby2]]]]]]]].
-  apply values_subtyping_split1 in Hsubx2.
-  apply values_subtyping_split2 in Hsuby2.
-  remove_bools_options.
-  (* Slightly difficult -- draw it out on paper *)
-  exists (ts2 ++ (take (size ts1) tsubx23)), (ts2' ++ (take (size ts1') tsuby23)), (drop (size ts1) tsubx23), (drop (size ts1') tsuby23); repeat rewrite -catA cat_take_drop.
-  repeat split => //; try by eapply values_subtyping_trans; eauto.
-  rewrite values_subtyping_cat => //; last by apply values_subtyping_size.
-  rewrite Hsub2 => /=.
-  by (do 2 (eapply values_subtyping_trans; eauto)).
-Qed.
-
-(* Trying to resolve subtyping goals in a non-breaking way. A different tactic is provided below that performs more destructive unfolds on instr and func subtyping relations. *)
-Ltac resolve_subtyping :=
-  repeat match goal with
-  | H: is_true ?b |-
-      context [ ?b ] =>
-      rewrite H => /=
-                    
-  | |- context [ ?t <t: ?t ] =>
-      rewrite value_subtyping_eq => //
-                                     
-  | |- context [ ?ts <ts: ?ts ] =>
-    rewrite values_subtyping_eq => //
-  | _: is_true (?ts1 <ts: ?ts1') |-
-      context [(?ts1 ++ ?ts2) <ts: (?ts1' ++ ?ts2')] =>
-      erewrite values_subtyping_cat; eauto; last by apply values_subtyping_size
-  | _: is_true (?ts1 <ts: ?ts2),
-    _: is_true ((?ts2 ++ ?ts3) <ts: ?ts4) |-
-       context [ (?ts1 ++ ?ts3) <ts: ?ts4 ] =>
-      erewrite values_subtyping_cat_trans; try by eauto
-                                                    
-  | |- context [ ?tf <tf: ?tf ] =>
-      rewrite func_subtyping_eq => //
-                                    
-  | |- context [ ?tf <ti: ?tf ] =>
-    try by apply instr_subtyping_eq => //
-                                     
-  | |- (Tf nil nil) <ti: (Tf ?ts0 ?ts0) =>
-    exists ts0, ts0, nil, nil; repeat split; repeat rewrite cats0 => //
-  | |- (Tf nil ?ts) <ti: (Tf ?ts0 (?ts0 ++ ?ts)) =>
-    exists ts0, ts0, nil, ts; repeat split; repeat rewrite cats0 => //
-  | |- (Tf ?ts nil) <ti: (Tf (?ts0 ++ ?ts) ?ts0) =>
-    exists ts0, ts0, ts, nil; repeat split; repeat rewrite cats0 => //
-  | |- (Tf ?ts1 ?ts2) <ti: (Tf (?ts0 ++ ?ts1) (?ts0 ++ ?ts2)) =>
-    exists ts0, ts0, ts1, ts2; repeat split; repeat rewrite cats0 => //
-
-  (* transitivities, up to a chain of length 3 *)
-  | H1: is_true (?a <t: ?b),
-    H2: is_true (?b <t: ?c) |-
-      context [ ?a <t: ?c ] =>
-      rewrite (value_subtyping_trans H1 H2) => /=
-  | H1: is_true (?a <t: ?b),
-    H2: is_true (?b <t: ?c),
-    H3: is_true (?c <t: ?d) |-
-      context [ ?a <t: ?d ] =>
-      rewrite (value_subtyping_trans (values_subtyping_trans H1 H2) H3) => /=
-                                                                             
-  | H1: is_true (?a <ts: ?b),
-    H2: is_true (?b <ts: ?c) |-
-      context [ ?a <ts: ?c ] =>
-      rewrite (values_subtyping_trans H1 H2) => /=
-  | H1: is_true (?a <ts: ?b),
-    H2: is_true (?b <ts: ?c),
-    H3: is_true (?c <ts: ?d) |-
-      context [ ?a <ts: ?d ] =>
-      rewrite (values_subtyping_trans (values_subtyping_trans H1 H2) H3) => /=
-                                                                             
-  | H1: (?a <ti: ?b),
-    H2: (?b <ti: ?c) |-
-      context [ ?a <ti: ?c ] =>
-      apply (instr_subtyping_trans H1 H2) => /=
-  | H1: (?a <ti: ?b),
-    H2: (?b <ti: ?c),
-    H3: (?c <ti: ?d) |-
-      context [ ?a <ti: ?d ] =>
-      apply (instr_subtyping_trans (instr_subtyping_trans H1 H2) H3) => /=
-
-  (* subtyping of empty *)
-  | H: is_true (?ts <ts: nil) |- _ =>
-      destruct ts => //; clear H
-  | H: is_true (nil <ts: ?ts) |- _ =>
-      destruct ts => //; clear H
-  end.
-
-Lemma values_subtyping_cat_suffix: forall ts1 ts2 ts3 ts4 tx ty n,
-    ts1 ++ ts2 = ts3 ++ ts4 ->
-    (tx <ts: ts2) ->
-    (drop n ts4 <ts: ty) ->
-    size tx = size ty ->
-    tx <ts: ty.
-Proof.
-  intros ??????? Hcat Hsubs1 Hsubs2 Hsize.
-  rewrite - (cat_take_drop n ts4) catA in Hcat.
-  apply concat_cancel_last_n in Hcat; last first.
-  { apply values_subtyping_size in Hsubs1, Hsubs2.
-    by lias.
-  }
-  remove_bools_options; subst.
-  by resolve_subtyping.
-Qed.
-
-Ltac extract_premise :=
-  repeat match goal with
-  | H: ?x = ?x -> _ |- _ =>
-    specialize (H erefl)
-  | H: forall x, ?x0 = x -> _ |- _ =>
-    try specialize (H _ erefl)
-  | H: forall x, [::?x0] = [::x] -> _ |- _ =>
-    try specialize (H _ erefl)
-  | H: forall x, [:: ?c ?x0] = [:: ?c x] -> _ |- _ =>
-    try specialize (H _ erefl)
-  | H: forall x y, [:: ?c ?x0 ?y0] = [:: ?c y x] -> _ |- _ =>
-    try specialize (H _ _ erefl)
-  | H: forall x y, [:: ?c ?x0 ?y0] = [:: ?c x y] -> _ |- _ =>
-    try specialize (H _ _ erefl)
-  | H: forall t ts, ?ts0 ++ [::?t0] = ts ++ [::t] -> _ |- _ =>
-    try specialize (H _ _ erefl)
-  | H: forall x y z, [:: ?c ?x0 ?y0 ?z0] = [:: ?c z y x] -> _ |- _ =>
-    try specialize (H _ _ _ erefl)
-  | H: forall x y, (Tf ?x0 ?y0) = (Tf y x) -> _ |- _ =>
-    try specialize (H _ _ erefl)
-  | H: forall x y, (Tf ?x0 ?y0) = (Tf x y) -> _ |- _ =>
-    try specialize (H _ _ erefl)
-  | H: exists t, ?P |- _ =>
-    let extr := fresh "extr" in
-    let Hextr := fresh "Hextr" in  
-    destruct H as [extr Hextr]
-  | H: ?P /\ ?Q |- _ =>
-    let Hconjl := fresh "Hconjl" in  
-    let Hconjr := fresh "Hconjr" in  
-    destruct H as [Hconjl Hconjr]
-  | _ => (repeat rewrite -> cats0 in * ); (repeat rewrite -> cat0s in * ); resolve_subtyping; subst
-    end.
-
-Lemma instr_subtyping_strengthen1: forall tx1 ty1 tx2 ty2 ts,
-    ((Tf tx1 ty1) <ti: (Tf tx2 ty2)) ->
-    (tx1 <ts: ts) ->
-    ((Tf ts ty1) <ti: (Tf tx2 ty2)).
-Proof.
-  intros.
-  unfold instr_subtyping in *; extract_premise.
-  exists extr, extr0, extr1, extr2.
-  by resolve_subtyping.
-Qed.
-
-Lemma instr_subtyping_strengthen2: forall tx1 ty1 tx2 ty2 ts,
-    ((Tf tx1 ty1) <ti: (Tf tx2 ty2)) ->
-    (ty2 <ts: ts) ->
-    ((Tf tx1 ty1) <ti: (Tf tx2 ts)).
-Proof.
-  intros ?????? Hsub.
-  unfold instr_subtyping in *; extract_premise.
-  apply values_subtyping_split2 in Hsub; remove_bools_options.
-  exists extr, (take (size extr0) ts), extr1, (drop (size extr0) ts); rewrite cat_take_drop.
-  by resolve_subtyping.
-Qed.
-
-Lemma instr_subtyping_weaken1: forall tx1 ty1 tx2 ty2 ts,
-    ((Tf tx1 ty1) <ti: (Tf tx2 ty2)) ->
-    (ts <ts: ty1) ->
-    ((Tf tx1 ts) <ti: (Tf tx2 ty2)).
-Proof.
-  intros.
-  unfold instr_subtyping in *; extract_premise.
-  exists extr, extr0, extr1, extr2.
-  by resolve_subtyping.
-Qed.
-
-Lemma instr_subtyping_weaken2: forall tx1 ty1 tx2 ty2 ts,
-    ((Tf tx1 ty1) <ti: (Tf tx2 ty2)) ->
-    (ts <ts: tx2) ->
-    ((Tf tx1 ty1) <ti: (Tf ts ty2)).
-Proof.
-  intros ?????? Hsub.
-  unfold instr_subtyping in *; extract_premise.
-  apply values_subtyping_split1 in Hsub; remove_bools_options.
-  exists (take (size extr) ts), extr0, (drop (size extr) ts), extr2; rewrite cat_take_drop.
-  by resolve_subtyping.
-Qed.
-
-Lemma num_subtyping: forall tn t,
-    (T_num tn <t: t) ->
-    t = T_num tn.
-Proof.
-  by intros; unfold value_subtyping in *; remove_bools_options.
-Qed.
-
-Lemma vec_subtyping: forall tn t,
-    (T_vec tn <t: t) ->
-    t = T_vec tn.
-Proof.
-  by intros; unfold value_subtyping in *; remove_bools_options.
-Qed.
-
-Lemma ref_subtyping: forall tn t,
-    (T_ref tn <t: t) ->
-    t = T_ref tn.
-Proof.
-  by intros; unfold value_subtyping in *; remove_bools_options.
-Qed.
-
-(* Only use this tactic if desperate *)
-Ltac simplify_subtyping :=
-  repeat match goal with
-  | H: is_true true |- _ => clear H
-  | H: ?x = ?x |- _ => clear H
-                              
-  | H: is_true (T_num ?t <t: ?t') |- _ =>
-    apply num_subtyping in H => //
-  | H: is_true (T_vec ?t <t: ?t') |- _ =>
-    apply vec_subtyping in H => //
-  | H: is_true (T_ref ?t <t: ?t') |- _ =>
-    apply ref_subtyping in H => //
-
-  | H: T_num ?t1 = T_num ?t2 |- _ =>
-    inversion H; subst; clear H
-                                
-  | H: T_vec ?t1 = T_vec ?t2 |- _ =>
-    inversion H; subst; clear H
-                                
-  | H: T_ref ?t1 = T_ref ?t2 |- _ =>
-    inversion H; subst; clear H
-      
-  (* Structural splits of values_typing *)
-  | H: is_true (?ts <ts: (?ts1 ++ ?ts2)) |- _ =>
-    let Hsubs1 := fresh "Hsubs1" in
-    let Hsubs2 := fresh "Hsubs2" in
-    apply values_subtyping_split1 in H; move/andP in H; destruct H as [Hsubs1 Hsubs2] => //
-  | H: is_true ((?ts1 ++ ?ts2) <ts: ?ts) |- _ =>
-    let Hsubs1 := fresh "Hsubs1" in
-    let Hsubs2 := fresh "Hsubs2" in
-    apply values_subtyping_split2 in H; move/andP in H; destruct H as [Hsubs1 Hsubs2] => //
-  | _ => (* real desperation mode *)
-        unfold instr_subtyping, func_subtyping in *; resolve_subtyping => //; remove_bools_options => //; extract_premise; subst => //; extract_listn; subst => //; simpl in *; remove_bools_options; subst => //
-  end.
-
-(* Auxiliary lemmas for composing types only knowing a principal type. In 1.0 the subtypings are simple concatenations, which made things a lot easier. *)
-Lemma instr_subtyping_compose_le: forall tx0 ty0 ty0' tz0 tx ty tz,
-    ((Tf tx0 ty0) <ti: (Tf tx ty)) ->
-    ((Tf ty0' tz0) <ti: (Tf ty tz)) ->
-    size ty0 <= size ty0' ->
-    ((Tf ((take (size ty0' - size ty0) ty0') ++ tx0) tz0) <ti: (Tf tx tz)) /\ (ty0 <ts: drop (size ty0' - size ty0) ty0').
-Proof.
-  intros ??????? Hsubi1 Hsubi2 Hsize.
-  simplify_subtyping.
-  specialize (values_subtyping_size Hconjl2) as Hsize'.
-  apply values_subtyping_split with (n := size ty0' - size ty0) in Hconjl2 as [Hsubs1 Hsubs2]; last by lias.
-  rewrite - (cat_take_drop (size ty0' - size ty0) extr1) catA in Hconjl.
-  specialize (values_subtyping_size Hconjr1) as Hsize''.
-  apply concat_cancel_last_n in Hconjl => //; remove_bools_options; subst; last by rewrite size_drop; lias.
-  simplify_subtyping; split => //.
-  exists (take (size extr) extr3), extr0, (drop (size extr) extr3 ++ extr5), extr2.
-  repeat split; resolve_subtyping => //.
-  - by rewrite catA cat_take_drop.
-  - rewrite values_subtyping_cat; first by resolve_subtyping.
-    apply values_subtyping_size in Hsubs3.
-    rewrite Hsubs3.
-    repeat rewrite size_takel; by lias.
-Qed.
-
-Lemma instr_subtyping_compose_ge: forall tx0 ty0 ty0' tz0 tx ty tz,
-    ((Tf tx0 ty0) <ti: (Tf tx ty)) ->
-    ((Tf ty0' tz0) <ti: (Tf ty tz)) ->
-    size ty0' <= size ty0 ->
-    ((Tf tx0 ((take (size ty0 - size ty0') ty0) ++ tz0)) <ti: (Tf tx tz)) /\ (drop (size ty0 - size ty0') ty0 <ts: ty0').
-Proof.
-  intros ??????? Hsubi1 Hsubi2 Hsize.
-  simplify_subtyping.
-  specialize (values_subtyping_size Hconjr1) as Hsize'.
-  apply values_subtyping_split with (n := size ty0 - size ty0') in Hconjr1 as [Hsubs1 Hsubs2]; last by lias.
-  rewrite - (cat_take_drop (size ty0 - size ty0') extr6) catA in Hconjl.
-  specialize (values_subtyping_size Hconjl2) as Hsize''.
-  apply concat_cancel_last_n in Hconjl => //; remove_bools_options; subst; last by rewrite size_drop; lias.
-  simplify_subtyping; split => //.
-  exists extr3, (take (size extr4) extr0), extr5, (drop (size extr4) extr0 ++ extr2).
-  repeat split; resolve_subtyping => //.
-  - by rewrite catA cat_take_drop.
-  - rewrite values_subtyping_cat; first by resolve_subtyping.
-    apply values_subtyping_size in Hsubs3.
-    rewrite - Hsubs3.
-    repeat rewrite size_takel; by lias.
-Qed.
-
-(* A few special cases *)
-Lemma instr_subtyping_compose_eq: forall tx0 ty0 ty0' tz0 tx ty tz,
-    ((Tf tx0 ty0) <ti: (Tf tx ty)) ->
-    ((Tf ty0' tz0) <ti: (Tf ty tz)) ->
-    size ty0 = size ty0' ->
-    ((Tf tx0 tz0) <ti: (Tf tx tz)) /\ (ty0 <ts: ty0').
-Proof.
-  intros ??????? Hsubi1 Hsubi2 Hsize.
-  specialize (instr_subtyping_compose_le Hsubi1 Hsubi2) as Hsub.
-  rewrite Hsize subnn take0 drop0 in Hsub.
-  apply Hsub; by lias.
-Qed.
-
-Lemma instr_subtyping_compose_nil1: forall tx0 ty0 tz0 tx ty tz,
-    ((Tf tx0 nil) <ti: (Tf tx ty)) ->
-    ((Tf ty0 tz0) <ti: (Tf ty tz)) ->
-    (Tf (ty0 ++ tx0) tz0) <ti: (Tf tx tz).
-Proof.
-  intros ?????? Hsubi1 Hsubi2.
-  specialize (instr_subtyping_compose_le Hsubi1 Hsubi2) as Hsub.
-  destruct Hsub as [Hsub _] => //.
-  uapply Hsub; do 2 f_equal => /=.
-  by rewrite subn0 take_size.
-Qed.
-
-Lemma instr_subtyping_compose_nil2: forall tx0 ty0 tz0 tx ty tz,
-    ((Tf tx0 ty0) <ti: (Tf tx ty)) ->
-    ((Tf nil tz0) <ti: (Tf ty tz)) ->
-    (Tf tx0 (ty0 ++ tz0)) <ti: (Tf tx tz).
-Proof.
-  intros ?????? Hsubi1 Hsubi2.
-  specialize (instr_subtyping_compose_ge Hsubi1 Hsubi2) as Hsub.
-  destruct Hsub as [Hsub _] => //.
-  uapply Hsub; do 2 f_equal => /=.
-  by rewrite subn0 take_size.
-Qed.
-
-Ltac unify_principal :=
-  repeat match goal with
-  | H1: (Tf ?ts1 ?ts2) <ti: (Tf ?tx ?ty),
-    H2: (Tf ?ts3 ?ts4) <ti: (Tf ?ty ?tz) |- _ =>
-    let Hprincipal := fresh "Hprincipal" in  
-    let Hsubs := fresh "Hsubs" in
-    (* syntactic sugar for matching 2 variables doesn't work in Ltac *)
-    match ts2 with
-    | nil => specialize (instr_subtyping_compose_nil1 H1 H2) as Hprincipal; clear H1 H2
-    | [::_] =>
-        match ts3 with
-        | nil => specialize (instr_subtyping_compose_nil2 H1 H2) as Hprincipal
-        | [::_] => specialize (instr_subtyping_compose_eq H1 H2) as [Hprincipal Hsubs] => //
-        | _ => specialize (instr_subtyping_compose_le H1 H2) as [Hprincipal Hsubs] => //
-        end; clear H1 H2
-    | [::_; _] =>
-        match ts3 with
-        | nil => specialize (instr_subtyping_compose_nil2 H1 H2) as Hprincipal
-        | [::_] => specialize (instr_subtyping_compose_ge H1 H2) as [Hprincipal Hsubs] => //
-        | [::_; _] => specialize (instr_subtyping_compose_eq H1 H2) as [Hprincipal Hsubs] => //
-        | _ => specialize (instr_subtyping_compose_le H1 H2) as [Hprincipal Hsubs] => //
-        end; clear H1 H2
-    | [::_; _; _] =>
-        match ts3 with
-        | nil => specialize (instr_subtyping_compose_nil2 H1 H2) as Hprincipal
-        | [::_; _] => specialize (instr_subtyping_compose_ge H1 H2) as [Hprincipal Hsubs] => //
-        | [::_; _] => specialize (instr_subtyping_compose_ge H1 H2) as [Hprincipal Hsubs] => //
-        | [::_; _; _] => specialize (instr_subtyping_compose_eq H1 H2) as [Hprincipal Hsubs] => //
-        | _ => specialize (instr_subtyping_compose_le H1 H2) as [Hprincipal Hsubs] => //
-        end; clear H1 H2
-    | _ => idtac "unification is too complicated"
-    end; try (move: Hprincipal; rewrite (lock instr_subtyping) /= -lock; move => Hprincipal)
-  | |- is_true (size _ <= size _) =>
-    try by repeat rewrite size_cat; lias
-  end.
-(* Some quality of life lemmas *)
-(* Upd: these lemmas are deprecated; it is encouraged to directly use subtyping rule. *)
-Lemma bet_weakening_empty_1: forall C es ts t2s,
-    be_typing C es (Tf [::] t2s) ->
-    be_typing C es (Tf ts (ts ++ t2s)).
-Proof.
-  move => C es ts t2s HType.
-  eapply bet_subtyping; eauto.
-  by resolve_subtyping.
-Qed.
-
-Lemma bet_weakening_empty_2: forall C es ts t1s,
-    be_typing C es (Tf t1s [::]) ->
-    be_typing C es (Tf (ts ++ t1s) ts).
-Proof.
-  move => C es ts t1s HType.
-  eapply bet_subtyping; eauto.
-  by resolve_subtyping.
-Qed.
-
-Lemma bet_weakening_empty_both: forall C es ts,
-    be_typing C es (Tf [::] [::]) ->
-    be_typing C es (Tf ts ts).
-Proof.
-  move => C es ts HType.
-  eapply bet_subtyping; eauto.
-  by resolve_subtyping.
-Qed.
-
 (** * More Advanced Lemmas **)
 
 Section Host.
 
 Context `{hfc: host_function_class}.
 
+Lemma values_typing_size: forall s vs ts,
+    values_typing s vs ts ->
+    size vs = size ts.
+Proof.
+  move => s vs ts Hvts.
+  by apply all2_size in Hvts.
+Qed.
+
 Lemma values_typing_length: forall s vs ts,
-    values_typing s vs = Some ts ->
+    values_typing s vs ts ->
     length vs = length ts.
 Proof.
   move => s vs ts Hvts.
-  apply those_length in Hvts.
-  by rewrite length_is_size size_map -length_is_size in Hvts.
+  apply all2_size in Hvts.
+  by repeat rewrite length_is_size.
 Qed.
 
 Lemma values_typing_cons_impl: forall s v t vs ts,
-    values_typing s (v :: vs) = Some (t :: ts) ->
-    value_typing s v = Some t /\
-    values_typing s vs = Some ts.
+    values_typing s (v :: vs) (t :: ts) ->
+    value_typing s v t /\
+    values_typing s vs ts.
 Proof.
   move => s v t vs ts Hvaltype.
-  by apply those_cons_impl in Hvaltype as [??].
+  simpl in Hvaltype; by remove_bools_options.
 Qed.
 
 Lemma values_typing_cat: forall s vs1 vs2 ts1 ts2,
-    values_typing s vs1 = Some ts1 ->
-    values_typing s vs2 = Some ts2 ->
-    values_typing s (vs1 ++ vs2) = Some (ts1 ++ ts2).
+    values_typing s vs1 ts1 ->
+    values_typing s vs2 ts2 ->
+    values_typing s (vs1 ++ vs2) (ts1 ++ ts2).
 Proof.
   move => s vs1 vs2 ts1 ts2.
   unfold values_typing.
   intros.
-  by rewrite map_cat; erewrite those_cat.
+  rewrite all2_cat; first by lias.
+  by apply all2_size in H.
 Qed.
 
 Lemma default_value_typing: forall s t v,
     default_val t = Some v ->
-    value_typing s v = Some t.
+    value_typing s v t.
 Proof.
   move => s t v Hval.
   destruct t, v => //; simpl in *; try inversion Hval; subst => //=.
   - by destruct n.
   - by destruct v0.
+  - by destruct r.
 Qed.
 
 Lemma default_values_typing: forall s ts vs,
     default_vals ts = Some vs ->
-    values_typing s vs = Some ts.
+    values_typing s vs ts.
 Proof.
   unfold default_vals, values_typing.
   setoid_rewrite <- those_those0.
   move => s; elim => /=; first by case.
   move => t ts IH vs Hdefaults; destruct vs => //; remove_bools_options => /=.
-  erewrite default_value_typing; eauto.
-  by erewrite IH; eauto.
+  by erewrite default_value_typing; eauto.
 Qed.
 
 (* Avoid changing everything to type or making other large-scale changes *)
@@ -1592,59 +1091,6 @@ Proof.
   apply const_es_exists in Hconst as [vcs Heq].
   assert (P vcs) as HP; first by (destruct Hexist as [? [-> HP]]; subst; apply v_to_e_inj in Heq; subst).
   by exists vcs.
-Qed.
-
-(** Typing lemmas **)
-
-(* A reformulation of [ety_a] that is easier to be used. *)
-Lemma ety_a': forall s C es ts,
-    es_is_basic es ->
-    be_typing C (to_b_list es) ts ->
-    e_typing s C es ts.
-Proof.
-  move => s C es ts HBasic HType.
-  replace es with (to_e_list (to_b_list es)).
-  - by apply ety_a.
-  - symmetry. by apply e_b_elim.
-Qed.
-
-Lemma et_weakening_empty_1: forall s C es ts t2s,
-    e_typing s C es (Tf [::] t2s) ->
-    e_typing s C es (Tf ts (ts ++ t2s)).
-Proof.
-  move => s C es ts t2s HType.
-  eapply ety_subtyping; eauto.
-  by resolve_subtyping.
-Qed.
-
-Lemma et_weakening_empty_2: forall s C es ts t2s,
-    e_typing s C es (Tf t2s nil) ->
-    e_typing s C es (Tf (ts ++ t2s) ts).
-Proof.
-  move => s C es ts t2s HType.
-  eapply ety_subtyping; eauto.
-  by resolve_subtyping.
-Qed.
-
-(* A convenient lemma to invert e_typing back to be_typing. *)
-Lemma et_to_bet: forall s C es tf,
-    es_is_basic es ->
-    e_typing s C es tf ->
-    be_typing C (to_b_list es) tf.
-Proof.
-  move => s C es tf HBasic HType.
-  dependent induction HType; basic_inversion => //.
-  + replace (to_b_list (to_e_list bes)) with bes => //.
-    by apply b_e_elim.
-  + rewrite to_b_list_concat.
-    apply basic_concat in HBasic.
-    move/andP in HBasic.
-    destruct HBasic as [Hbes Hbe].
-    eapply bet_composition.
-    * by eapply IHHType1 => //.
-    * by eapply IHHType2 => //.
-  + apply IHHType in HBasic.
-    by eapply bet_subtyping; eauto.
 Qed.
 
 (************ these come from the certified itp *************)
